Pass WIP

Iris/Iris/ProgramLogic/TotalAdequacy.lean
@@ -16,42 +16,19 @@ open Language Language.Notation
 
 /-! ## Total adequacy -/
 
-/-- Strong normalization for `step`. -/
-def StronglyNormalizing {α : Type _} (step : α → α → Prop) (x : α) : Prop :=
-  Acc (flip step) x
-
-namespace StronglyNormalizing
-
-theorem intro {α : Type _} {step : α → α → Prop} {x : α}
-    (H : ∀ y, step x y → StronglyNormalizing step y) :
-    StronglyNormalizing step x := Acc.intro x H
-
-theorem map {α β : Type _} {stepα : α → α → Prop}
-    {stepβ : β → β → Prop} (f : β → α)
-    (Hlift : ∀ x y, stepβ x y → stepα (f x) (f y))
-    {x : β} (H : StronglyNormalizing stepα (f x)) :
-    StronglyNormalizing stepβ x :=
-  Subrelation.accessible (fun h => Hlift _ _ h) (InvImage.accessible f H)
-
-end StronglyNormalizing
-
-variable {Expr State Obs Val : Type _} [Λ : Language Expr State Obs Val]
-
 section ThreadPool
 
+variable {Expr State Obs Val : Type _} [Λ : Language Expr State Obs Val]
 variable {hlc : HasLC} {GF : BundledGFunctors}
 variable [ι : IrisGS_gen hlc Expr GF]
 
 local instance : OFE (List Expr) := OFE.ofDiscrete _
-
 local instance list_nonexpansive (Ψ : List Expr → IProp GF) : NonExpansive Ψ :=
   ⟨fun _ _ _ hxy => hxy ▸ .rfl⟩
+local instance : OFE Val := OFE.ofDiscrete _
 
 namespace twptp
 
-local instance : OFE CoPset := OFE.ofDiscrete _
-local instance : OFE Expr := OFE.ofDiscrete _
-local instance : OFE Val := OFE.ofDiscrete _
 
 private theorem step_append_inv (r₁ r₂ : List Expr) {t' : List Expr} {σ₁ σ₂ : State} {κ : List Obs} :
     (r₁ ++ r₂, σ₁) -<κ>->ₜₚ (t', σ₂) →
@@ -70,12 +47,12 @@ private theorem step_append_inv (r₁ r₂ : List Expr) {t' : List Expr} {σ₁ 
 
 /-- One unfolding of the total thread-pool predicate. -/
 @[rocq_alias twptp_pre]
-def pre (X : List Expr → IProp GF) (t₁ : List Expr) : IProp GF := iprop(
+def pre (X : List Expr → IProp GF) (t₁ : List Expr) : IProp GF := iprop%
   ∀ (t₂ : List Expr) (σ₁ : State) (ns : Nat) (κ κs : List Obs)
       (σ₂ : State) (nt : Nat),
     ⌜(t₁, σ₁) -<κ>->ₜₚ (t₂, σ₂)⌝ -∗
     stateInterp σ₁ ns κs nt ={⊤}=∗
-      ∃ nt', ⌜κ = []⌝ ∗ stateInterp σ₂ (ns + 1) κs nt' ∗ X t₂)
+      ∃ nt', ⌜κ = []⌝ ∗ stateInterp σ₂ (ns + 1) κs nt' ∗ X t₂
 
 instance pre_mono_inst : BIMonoPred (pre (ι := ι)) where
   mono_pred := by
@@ -90,37 +67,37 @@ instance pre_mono_inst : BIMonoPred (pre (ι := ι)) where
 
 @[rocq_alias twptp_pre_mono]
 theorem pre_mono (X Y : List Expr → IProp GF) :
-    ⊢ □ (∀ t, X t -∗ Y t) -∗
-      ∀ t, pre (ι := ι) X t -∗ pre (ι := ι) Y t :=
-  mono_pred (F := pre (ι := ι))
+    □ (∀ t, X t -∗ Y t) -∗
+      ∀ t, pre X t -∗ pre Y t := mono_pred
 
 /-- Total weakest precondition for a thread pool. -/
 @[rocq_alias twptp]
 def get (t : List Expr) : IProp GF :=
-  bi_least_fixpoint (pre (ι := ι)) t
+  bi_least_fixpoint pre t
 
-instance get_ne : NonExpansive (get (ι := ι)) :=
-  list_nonexpansive _
+instance get_ne : NonExpansive (get (ι := ι)) := list_nonexpansive _
 
 @[rocq_alias twptp_unfold]
 theorem unfold (t : List Expr) :
-    get (ι := ι) t ⊣⊢ pre (ι := ι) (get (ι := ι)) t :=
-  BI.equiv_iff.1 (least_fixpoint_unfold (pre (ι := ι)))
+    get (ι := ι) t ⊣⊢ pre get t :=
+  BI.equiv_iff.1 (least_fixpoint_unfold pre)
 
 @[rocq_alias twptp_ind]
 theorem induction (Ψ : List Expr → IProp GF) :
-    (⊢ □ ∀ t, pre (ι := ι) (fun t => iprop(Ψ t ∧ get (ι := ι) t)) t -∗ Ψ t) →
-    ⊢ ∀ t, get (ι := ι) t -∗ Ψ t := fun H => by
-  simpa [get, BIBase.EmpValid] using H.trans (BI.wand_entails (least_fixpoint_ind (F := pre (ι := ι)) (Φ := Ψ)))
+    ⊢ (□ ∀ t, pre (fun t => iprop(Ψ t ∧ get t)) t -∗ Ψ t) →
+    ∀ t, get t -∗ Ψ t := by
+  iintro #IH %t H
+  unfold get
+  iapply least_fixpoint_ind $$ [$] [$]
+
 
 @[rocq_alias twptp_Permutation]
 theorem permutation {t₁ t₁' : List Expr} (Hp : t₁.Perm t₁') :
-    get (ι := ι) t₁ ⊢ get (ι := ι) t₁' := by
+    get (ι := ι) t₁ ⊢ get t₁' := by
   iintro Ht
-  iapply induction (fun t : List Expr => iprop(∀ t', ⌜t.Perm t'⌝ -∗ get (ι := ι) t'))
-    (ι := ι) ?_ $$ %t₁ Ht %t₁' %Hp
+  iapply induction (fun t : List Expr => iprop(∀ t', ⌜t.Perm t'⌝ -∗ get t')) $$ [] %t₁ Ht %t₁' %Hp
   iintro !> %t Hpre %t' %Htt'
-  simp only [(twptp.unfold (ι := ι) t').to_eq, pre]
+  simp only [(twptp.unfold t').to_eq, pre]
   iintro %t₂ %σ₁ %ns %κ %κs %σ₂ %nt %Hstep Hσ
   obtain ⟨t₂', H₂perm, Hstep'⟩ := Language.perm_of_step Htt'.symm Hstep
   imod Hpre $$ %_ %_ %_ %_ %_ %_ %_ %Hstep' Hσ with ⟨%nt', %hκ, Hσ, ⟨HIH, -⟩⟩
@@ -129,17 +106,14 @@ theorem permutation {t₁ t₁' : List Expr} (Hp : t₁.Perm t₁') :
 
 @[rocq_alias twptp_app]
 theorem app (t₁ t₂ : List Expr) :
-    get (ι := ι) t₁ -∗ get (ι := ι) t₂ -∗ get (ι := ι) (t₁ ++ t₂) := by
-  let Ψ₁ := fun t₁ : List Expr => iprop(
-    ∀ t₂, get (ι := ι) t₂ -∗ get (ι := ι) (t₁ ++ t₂))
+    get (ι := ι) t₁ -∗ get t₂ -∗ get (t₁ ++ t₂) := by
+  let Ψ₁ := fun t₁ : List Expr => iprop% ∀ t₂, get (ι := ι) t₂ -∗ get (t₁ ++ t₂)
   iintro H₁
-  iapply induction Ψ₁ (ι := ι) ?_ $$ %t₁ H₁ %t₂
-  let Ψ₂ := fun t₂ : List Expr => iprop(
-    ∀ t₁, pre (ι := ι)
-      (fun t => iprop(Ψ₁ t ∧ get (ι := ι) t)) t₁ -∗
-      get (ι := ι) (t₁ ++ t₂))
+  iapply induction Ψ₁ $$ [] %t₁ H₁ %t₂
+  let Ψ₂ := fun t₂ : List Expr => iprop%
+    ∀ t₁, pre (fun t => iprop(Ψ₁ t ∧ get t)) t₁ -∗ get (t₁ ++ t₂)
   iintro !> %u₁ Hu₁ %u₂ Hu₂
-  iapply induction Ψ₂ (ι := ι) ?_ $$ %u₂ Hu₂ %u₁ Hu₁
+  iapply induction Ψ₂ $$ [] %u₂ Hu₂ %u₁ Hu₁
   iintro !> %r₂ Hr₂ %r₁ Hr₁
   simp only [(twptp.unfold (ι := ι) (r₁ ++ r₂)).to_eq, pre]
   iintro %t' %σ₁ %ns %κ %κs %σ₂ %nt %Hstep Hσ
@@ -164,69 +138,61 @@ private theorem get_nil : ⊢ get (ι := ι) ([] : List Expr) := by
   iintro %t₂ %σ₁ %ns %κ %κs %σ₂ %nt %Hstep
   grind [List.append_eq_nil_iff]
 
-private theorem bigSepL_get_singleton (es : List Expr) :
-    ([∗list] e ∈ es, get (ι := ι) [e]) ⊢ get (ι := ι) es :=
-  List.rec (get_nil (ι := ι)) (fun e es IH =>
-    (BI.sep_mono_right IH).trans (BI.wand_elim (BI.wand_entails (app [e] es (ι := ι))))) es
-
 @[rocq_alias twp_twptp]
 theorem of_twp (s : Stuckness) (e : Expr) (Φ : Val → IProp GF) :
-    WP e @ s ; ⊤ [{ Φ }] ⊢ get (ι := ι) [e] := by
-  let Ψ := fun (E : CoPset) (e : Expr) (_ : Val → IProp GF) => iprop(
-    ⌜E = ⊤⌝ -∗ get (ι := ι) [e])
+    WP e @ s ; ⊤ [{ Φ }] ⊢ get [e] := by
+  let Ψ := fun (E : CoPset) (e : Expr) (_ : Val → IProp GF) => iprop(⌜E = ⊤⌝ -∗ get (ι := ι) [e])
   letI : NonExpansive
       (fun x : twp.Internal.Args Expr Val GF => Ψ x.1 x.2.1 x.2.2) :=
     ⟨fun _ _ _ ⟨hE, he, _⟩ => hE ▸ he ▸ .rfl⟩
   iintro He
   iapply twp.induction s Ψ (ι := ι) $$ [] He %rfl
-  iintro !> %e %E %Φ
-  cases he : toVal e
-  all_goals
-    simp only [twp.pre, he]
-    iintro Hpre %hE
-    simp only [hE, (twptp.unfold (ι := ι) [e]).to_eq, pre]
-    iintro %t₂ %σ₁ %ns %κ %κs %σ₂ %nt %Hstep
-    obtain ⟨e₂, efs, Hprim, rfl⟩ :
-        ∃ e₂ efs, (e, σ₁) -<κ>-> (e₂, σ₂, efs) ∧ t₂ = e₂ :: efs := by
+  iintro !> %e %E %Φ IH %hE
+  subst hE
+  simp only [(unfold [e]).to_eq, twp.pre, pre]
+  iintro %t₂ %σ₁ %ns %κ %κs %σ₂ %nt %Hstep Hσ₁
+  obtain ⟨e₂, efs, Hprim, rfl⟩ :
+      ∃ e₂ efs, (e, σ₁) -<κ>-> (e₂, σ₂, efs) ∧ t₂ = e₂ :: efs := by
       grind [List.append_eq_singleton_iff]
-  next =>
-    iintro Hσ
-    imod Hpre $$ Hσ with ⟨%_, Hpre⟩
+  cases he: toVal e <;> dsimp only []
+  · imod IH $$ Hσ₁ with ⟨%_, Hpre⟩
     imod Hpre $$ %κ %e₂ %σ₂ %efs %Hprim with ⟨%hκ, Hσ, ⟨IH₂, -⟩, Hefs⟩
     iframe %hκ Hσ
     rw [show e₂ :: efs = [e₂] ++ efs by simp]
     iapply app [e₂] efs (ι := ι) $$ (IH₂ $$ %rfl)
-    iapply (BigSepL.bigSepL_mono_of_forall ((sep_intro_emp_valid_left (pure_intro rfl) and_elim_l).trans
-      (wand_elim_swap .rfl))).trans (bigSepL_get_singleton efs (ι := ι)) $$ Hefs
-  next => simpa [he] using Language.val_stuck Hprim
+    clear Hprim Hstep
+    iinduction efs with
+    | nil => iapply get_nil
+    | cons e ef IH =>
+      isimp at Hefs
+      icases Hefs with ⟨⟨IH', -⟩, Hefs⟩
+      ieval (rewrite [← List.singleton_append])
+      iapply app [e] ef $$ [IH']
+      · iapply IH' $$ %rfl
+      iapply IH $$ Hefs
+  · simpa [he] using Language.val_stuck Hprim
 
 end twptp
 
 @[rocq_alias twptp_total]
 theorem twptp_total (t : List Expr) (σ : State) (ns nt : Nat) :
     stateInterp σ ns ([] : List Obs) nt -∗ twptp.get (ι := ι) t
-      ={⊤|}=∗ ⌜StronglyNormalizing
-        (Language.ErasedStep (Expr := Expr) (State := State) (Obs := Obs))
-        (t, σ)⌝ := by
-  let Ψ := fun t : List Expr => iprop(
+      ={⊤|}=∗ ⌜Relation.StronglyNormalizing ErasedStep (t, σ)⌝ := by
+  let Ψ := fun t : List Expr => iprop%
     ∀ (σ : State) (ns nt : Nat),
-      StateInterp.stateInterp (GF := GF) σ ns ([] : List Obs) nt -∗
-      |={⊤|}=> ⌜StronglyNormalizing
-        (Language.ErasedStep (Expr := Expr) (State := State) (Obs := Obs))
-        (t, σ)⌝)
+      StateInterp.stateInterp (GF := GF) σ ns ([] : List Obs) nt ={⊤|}=∗
+         ⌜Relation.StronglyNormalizing ErasedStep (t, σ)⌝
   iintro Hσ Ht
-  iapply twptp.induction Ψ (ι := ι) ?_ $$ %t Ht %σ %ns %nt Hσ
-  iintro !> %t
-  unfold twptp.pre
-  iintro Hpre %σ %ns %nt Hσ
-  iapply fupd_finally_mono (pure_mono StronglyNormalizing.intro)
+  iapply twptp.induction Ψ $$ [] %t Ht %σ %ns %nt Hσ
+  iintro !> %t IH %σ %ns %nt Hσ
+  iapply fupd_finally_mono (pure_mono (Acc.intro _))
   iintro %⟨t₂, σ₂⟩ %⟨κ, Hstep⟩
-  imod Hpre $$ %_ %_ %_ %_ %_ %_ %_ %Hstep Hσ with ⟨%nt', %hκ, Hσ, ⟨IH, -⟩⟩
+  unfold twptp.pre
+  imod IH $$ %_ %_ %_ %_ %_ %_ %_ %Hstep Hσ with ⟨%nt', %hκ, Hσ, ⟨IH, -⟩⟩
   iapply IH $$ %σ₂ %(ns + 1) %nt' Hσ
 
 end ThreadPool
 
-omit Λ in
 /-- Total adequacy for thread-pool reduction. -/
 @[rocq_alias twp_total]
 theorem twp_total {hlc : HasLC} {GF : BundledGFunctors}
@@ -242,42 +208,15 @@ theorem twp_total {hlc : HasLC} {GF : BundledGFunctors}
             stateI σ ns obs nt ⊢ |={∅}=> stateI σ (ns + 1) obs nt),
         let _ : IrisGS_gen hlc Expr GF :=
           .mk (toStateInterp := ⟨stateI⟩) numLatersPerStep forkPost mono
-        iprop(stateI σ n [] 0 ∗
-          (£ m -∗ WP e @ s ; ⊤ [{ Φ }]))) :
-    StronglyNormalizing
-      (Language.ErasedStep (Expr := Expr) (State := State) (Obs := Obs))
-      ([e], σ) := by
-  refine pure_soundness (PROP := IProp GF) (fupd_finally_soundness hlc m ⊤ _ ?_)
+        iprop% stateI σ n [] 0 ∗ (£ m -∗ WP e @ s ; ⊤ [{ Φ }])) :
+    Relation.StronglyNormalizing ErasedStep ([e], σ) := by
+  refine pure_soundness (PROP := IProp GF) ?_
+  refine (fupd_finally_soundness hlc m ⊤ _ ?_)
   iintro %Hinv Hcred
-  imod Hwp with
-    ⟨%stateI, %numLatersPerStep, %forkPost, %mono, Hσ, Htwp⟩
-  letI iG : IrisGS_gen hlc Expr GF :=
-    .mk (toStateInterp := ⟨stateI⟩) numLatersPerStep forkPost mono
-  iapply twptp_total [e] σ n 0 (ι := iG) $$ Hσ
-  iapply twptp.of_twp s e Φ (ι := iG) $$ (Htwp $$ Hcred)
-
-/-- Erased single-expression reduction. -/
-def ExprErasedStep : Expr × State → Expr × State → Prop
-  | (e₁, σ₁), (e₂, σ₂) =>
-      ∃ (κ : List Obs) (efs : List Expr), (e₁, σ₁) -<κ>-> (e₂, σ₂, efs)
-
-/-- A language whose primitive steps do not fork. -/
-class LanguageNoFork (Expr State Obs Val : Type _)
-    [Language Expr State Obs Val] : Prop where
-  no_fork {e₁ e₂ : Expr} {σ₁ σ₂ : State} {κ : List Obs} {efs : List Expr} :
-    (e₁, σ₁) -<κ>-> (e₂, σ₂, efs) → efs = []
-
-/-- Derive single-expression normalization from thread-pool normalization. -/
-theorem stronglyNormalizing_expr_of_threadPool
-    [LanguageNoFork Expr State Obs Val] {e : Expr} {σ : State}
-    (H : StronglyNormalizing
-      (Language.ErasedStep (Expr := Expr) (State := State) (Obs := Obs))
-      ([e], σ)) :
-    StronglyNormalizing
-      (ExprErasedStep (Expr := Expr) (State := State) (Obs := Obs))
-      (e, σ) :=
-  StronglyNormalizing.map (fun ρ : Expr × State => ([ρ.1], ρ.2))
-    (fun _ _ ⟨κ, efs, Hstep⟩ => ⟨κ, by simpa [LanguageNoFork.no_fork Hstep] using Step.atomic Hstep [] []⟩) H
+  imod Hwp with ⟨%stateI, %numLatersPerStep, %forkPost, %mono, Hσ, Htwp⟩
+  letI iG : IrisGS_gen hlc Expr GF := .mk (toStateInterp := ⟨stateI⟩) numLatersPerStep forkPost mono
+  iapply twptp_total [e] _ n _ $$ Hσ
+  iapply twptp.of_twp s e Φ $$ (Htwp $$ Hcred)
 
 end
 end Iris.ProgramLogic
